lectures/Rocq/notes_07_types.v
@@ -1,0 +1,1559 @@
+Require Import Coq.Strings.String Coq.Init.Nat Lia.
+
+(** * Simply Typed Lambda Calculus **)
+
+(** In this section, we formalize type safety for the Simply Typed
+    Lambda Calculus (STLC), adding a few simple extensions to the
+    language.
+
+    The extensions we consider are:
+
+    - Type of booleans 
+    - Type of natural numbers
+    - Sum type
+    - Product type
+
+
+    Each type comes with its own operations. We first give an informal
+    account of the added contructs and we describe its static and
+    dynamic semantics. *)
+
+(** ** Booleans *)
+
+(** - Type: [Bool]
+
+- Description: The usual boolean datatype, representing truth values.
+
+- Constructors: [true] and [false]
+
+- Values: [true] and [false]
+
+- Elimination form: Conditional expressions of the form [if b then e1 else e2] 
+
+- Static semantics:
+
+
+<<
+
+      --------------------(Ty_true)
+         Γ ⊢ true : Bool
+
+
+      --------------------(Ty_false)
+        Γ ⊢ false : Bool
+
+
+       Γ ⊢ b : Bool   Γ ⊢ a1 : A   Γ ⊢ a2 : A  
+      -----------------------------------------(Ty_if)
+           Γ  ⊢ if b then e1 else e2 : A
+
+>>
+
+
+- Dynamic semantics:
+
+<<
+      ----------------------------------(step_if_true)
+        if true then e1 else e2 --> e1
+
+
+      ----------------------------------(step_if_false)
+        if false then e1 else e2 --> e2
+
+
+                            e --> e'
+      ----------------------------------------------------(step_if)
+        if e then e1 else e2 -->  if e' then e1 else e2
+>>
+*)
+
+(** ** Natural Numbers *)
+
+(** - Type: [Nat]
+
+- Description: Non-negative integers.
+
+- Constructors: 0,1,2,3, etc.
+
+- Values: 0,1,2,3, etc.
+
+- Elimination form: We don't add explicit elimination forms, like a
+  case analysis construct for natural numbers. This behavior can be
+  simulated with the binary operators and the if-the-else construct.
+
+- Static semantics:
+<<
+      --------------------(Ty_nat)
+            Γ ⊢ n : Nat
+>>
+
+- Dynamic semantics: See binary operators below.
+
+*)
+
+(** *** Binary and Unary Operators on Booleans and Naturals *)
+
+(** To make the language easier to use we add a number of primitive
+    binary and unary operators as primitives. These are:
+
+    - Addition (+), subtraction (-), multiplication ( * )
+
+    - Disjunction (||), conjunction (&&)
+
+    - Less-than (<), equal (=)
+
+    - Negation (~)  
+
+
+- Static semantics:
+
+<<
+             Γ ⊢ e1 : Nat      Γ ⊢ e2 : Nat
+      -----------------------------------------(Ty_Bop_nat)   if ⊕ ∈ {+, -, *} 
+                  Γ ⊢ e1 ⊕ e2 : Nat
+
+
+             Γ ⊢ e1 : Bool     Γ ⊢ e2 : Bool
+      -----------------------------------------(Ty_Bop_bool)  if ⊕ ∈ {&&, ||} 
+                  Γ ⊢ e1 ⊕ e2 : Bool
+
+
+             Γ ⊢ e1 : Nat      Γ ⊢ e2 : Nat
+      -----------------------------------------(Ty_Bop_cmp)   if ⊕ ∈ {<, =} 
+                  Γ ⊢ e1 ⊕ e2 : Bool
+
+
+                   Γ ⊢ e : Bool
+      -----------------------------------------(Ty_Uop) 
+                  Γ ⊢ ~ e : Bool
+>>
+
+- Dynamic semantics:
+
+  Let ⊕ be a boolean operator, we denote its interpretation as [⊕]. 
+
+<<
+      ---------------------------(step_bop_nat)    if ⊕ ∈ {+, -, *}
+        n1 ⊕ n2  --> n1 [⊕] n2
+
+
+      ---------------------------(step_bop_bool)   if ⊕ ∈ {&&, ||}
+        b1 ⊕ b2  --> b1 [⊕] b2
+
+
+      ---------------------------(step_bop_cmp)    if ⊕ ∈ {<, =}
+        n1 ⊕ n2  --> n1 [⊕] n2
+
+
+              e1 --> e1'
+      ---------------------------(step_bop_l) 
+        e1 ⊕ e2  --> e1' ⊕ e2
+
+
+              value v1
+              e1 --> e2'
+      ---------------------------(step_bop_r) 
+        v1 ⊕ e2'  --> v1 ⊕ e2'
+
+
+
+
+      ---------------------------(step_uop_true)
+        ~ true  -->  false
+
+
+      ---------------------------(step_uop_bool)
+        ~ false  -->  true
+
+
+
+               e --> e'
+      ---------------------------(step_uop)
+            ~ e  --> ~ e'
+>>
+
+*)
+
+(** ** Unit type *)
+
+(** - Type: [Unit]
+
+- Description: A type with one value and no operations on it.
+
+- Constructors: [unit]
+
+- Values: [unit]
+
+- Elimination form: None. 
+
+- Static semantics:
+
+
+<<
+
+      --------------------(Ty_unit)
+         Γ ⊢ unit : Unit
+
+>>
+
+
+- Dynamic semantics: No added rules.
+*)
+
+(** ** Product Type *)
+
+(** - Type: [A * B] where [A] and [B] are types.
+
+- Description: A pair of values of types [A] and [B].
+
+- Constructors: [(a, b)] where [a] and [b] are terms of the respective type.
+
+- Values: [(a, b)] when [a] and [b] are values.
+
+- Elimination form: First projection [e.1] and second projection [e.2]
+
+- Static semantics:
+
+
+<<
+
+               Γ ⊢ e1 : A      Γ ⊢ e2 : B
+      -----------------------------------------(Ty_Pair) 
+                Γ ⊢ (e1, e2) : A * B
+
+
+                  Γ ⊢ e : A * B
+      -----------------------------------------(Ty_Fst) 
+                   Γ ⊢ e.1 : A
+
+
+                  Γ ⊢ e : A * B
+      -----------------------------------------(Ty_Sbd) 
+                   Γ ⊢ e.2 : B
+
+>>
+
+- Dynamic semantics:
+<<
+
+          value v1    value v2
+      ---------------------------(step_fst_v)
+           (v1, v2).1 --> v1
+
+
+          value v1    value v2
+      ---------------------------(step_snd_v)
+           (v1, v2).2 --> v2
+
+
+
+                t --> t'
+      ---------------------------(step_fst)
+              t.1 --> t'.1
+
+                t --> t'
+      ---------------------------(step_fst)
+              t.2 --> t'.2
+
+
+              e1 --> e1'
+      ---------------------------(step_pair_l)
+        (e1, e2) --> (e1', e2)
+
+
+              value v1
+              e1 --> e2'
+      ---------------------------(step_pair_l)
+        (v1, e2) --> (v1, e2')
+>>
+*)
+
+(** ** Sum Type *)
+
+(** - Type: [A + B] where [A] and [B] are types.
+
+- Description: A value of a sum type is either a value of type [A],
+  wrapped in the constructor [inl], or value of type [B], wrapped in
+  the constructor [inlr]. A generalization of the sum type is tagged
+  union types (or variants).
+
+- Constructors: [inl a] or [inr b], where [a] and [b] are terms of the
+  respective type. 
+
+- Values: [inl a] or [inr b], when [a] and [b] are values.
+
+- Elimination form: Case analysis of the form [case e of | inl y1 => e1 | inr y2 => e2].
+  At each arm of the case the binders [y1] and [y2] bind the inner
+  value of the sum constructors [inl] and [inr].
+
+- Static semantics:
+
+
+<<
+
+                 Γ ⊢ e1 : A
+      -----------------------------------------(Ty_Inl)
+              Γ ⊢ inl e1 : A + B
+
+
+                 Γ ⊢ e2 : B
+      -----------------------------------------(Ty_Inr)
+              Γ ⊢ inl e2 : A + B
+
+
+                      Γ ⊢ e : A + B
+          Γ, y1 : A ⊢ e1 : C      Γ, y2 : B ⊢ e2 : C
+      ------------------------------------------------------(Ty_Fst)
+        Γ ⊢ case e of | inl y1 => e1 | inr y2 => e2 : C
+>>
+
+- Dynamic semantics:
+<<
+                                  value v
+      --------------------------------------------------------------------(step_case_inl)
+        case inl v of | inl y1 => e1 | inr y2 => e2  --> [y1 := v]e1
+
+
+                                  value v
+      --------------------------------------------------------------------(step_case_inr)
+        case inr v of | inl y1 => e1 | inr y2 => e2  --> [y2 := v]e1
+
+
+                                  t --> t'
+      ----------------------------------------------------------------------------------------(step_case)
+        case t of | inl y1 => e1 | inr y2 => e2 --> case t' of | inl y1 => e1 | inr y2 => e2
+
+
+
+              e1 --> e1'
+      ---------------------------(step_inl)
+          inl e1 --> inl e1'
+
+
+              e2 --> e2'
+      ---------------------------(step_inr)
+          inl e2 --> inl e2'
+>>
+*)
+
+(** ** Let binding *)
+
+(** We also add let bindings as a primitive of the language and not as
+    a derived form (syntactic sugar).
+
+- Static semantics:
+
+<<
+        Γ ⊢ e1 : A    Γ, x : A  ⊢ e2 : B
+      ------------------------------------(Ty_let)
+              Γ ⊢ let x = e1 in e2 : B
+>>
+
+
+- Dynamic semantics:.
+<<
+                        value v1 
+      --------------------------------------------(step_let_value)
+            let x := v1 in e2 --> e2[x := v1]
+
+
+                       e1 --> e1'
+      --------------------------------------------(step_let)
+        let x := e1 in e2 --> let x := e1' in e2
+
+>>
+*)
+
+
+(** ** Syntax **)
+
+(** We start the formalization by defining the abstract syntax of the extended STLC. *)
+
+(** The abstract syntax of types. *)
+Inductive type : Type :=
+| Arrow : type -> type -> type
+| Nat   : type
+| Bool  : type
+| Unit  : type
+| Sum   : type -> type -> type
+| Prod  : type -> type -> type.
+
+(** Binary Operators. *)
+
+(** To make definitions less verbose we group all binary operators
+    under the same type [bop]. This allows us to handle them
+    uniformly when possible. *)
+Inductive bop :=
+(* arithmetic operators *)
+| Plus | Minus | Mult
+(* boolean operators *)
+| And | Or
+(* comparison operators *)
+| Lt | Eq.
+
+(** Unary Operators. *)
+Inductive uop :=
+| Neg.
+
+(** The abstract syntax of terms. *)
+Inductive term : Type :=
+(* Pure STLC fragment with functions, applications, and variables. *)
+| T_App : term -> term -> term
+| T_Lambda : string -> type -> term -> term
+| T_Var : string -> term
+(* Let *)
+| T_Let : string -> term -> term -> term                      
+(* Booleans *)
+| T_Bool : bool -> term
+(* If *)
+| T_If : term -> term -> term -> term
+(* Natural Numbers *)
+| T_Nat : nat -> term
+(* Binary Operators *)
+| T_BOp : bop -> term -> term -> term
+(* Unary Operatos *)
+| T_UOp : uop -> term -> term
+(* Pairs *)
+| T_Pair : term -> term -> term
+| T_Fst : term -> term
+| T_Snd : term -> term
+(* Sums *)
+| T_Inl : type -> term -> term
+| T_Inr : type -> term -> term
+| T_Case : term -> string -> term -> string -> term -> term
+.
+
+
+(** As usual, we define familiar syntax for terms of the object
+    language. Terms of the object language are written inside
+    quotations [ <[ t ]> ]. Standalone types of the object language
+    are written inside quotations [ <[[ t ]]> ]. In order to be able
+    to write Coq terms inside object language quotations, introduce
+    anti-quotations using curly braces [ { t } ]. Inside
+    anti-quotations, we can escape the syntax of the object language
+    and directly use the standard Coq syntax to write terms. *)
+
+Declare Scope ML_scope.
+
+Declare Custom Entry ML.
+Declare Custom Entry ML_ty.
+
+Notation "<[ e ]>" := e (e custom ML at level 99) : ML_scope.
+Notation "( x )" := x (in custom ML, x at level 99).
+Notation "x" := x (in custom ML at level 0, x constr at level 0).
+
+
+Notation "<[[ e ]]>" := e (e custom ML_ty at level 99) : ML_scope.
+Notation "( x )" := x (in custom ML_ty, x at level 99).
+Notation "x" := x (in custom ML_ty at level 0, x constr at level 0).
+
+(** Types *)
+
+Notation "S + T" := (Sum S T) (in custom ML_ty at level 3, left associativity).
+Notation "X * Y" :=
+  (Prod X Y) (in custom ML_ty at level 2, X custom ML_ty, Y custom ML_ty at level 0).
+Notation "S -> T" := (Arrow S T) (in custom ML_ty at level 50, right associativity).
+
+(** Terms *)
+
+Notation "x y" := (T_App x y) (in custom ML at level 1, left associativity).
+
+Notation "'fun'  x ':' T  '->' y" := (T_Lambda x T y) (in custom ML at level 90,
+                                           x at level 99,
+                                           T custom ML at level 99,
+                                           y custom ML at level 99,
+                                           left associativity) : ML_scope.
+
+Notation "'let' x ':=' y 'in' z" := (T_Let x y z) (in custom ML at level 90,
+                                          x at level 99,
+                                          y custom ML at level 100,
+                                          z custom ML at level 100, left associativity) : ML_scope.
+
+Notation "'if' x 'then' y 'else' z" :=
+  (T_If x y z)
+    (in custom ML at level 89, x at level 99,
+        y at level 99, z at level 99) : ML_scope.
+
+Notation "x <= y" := (T_BOp Or (T_BOp Lt x y) (T_BOp Eq x y))
+                       (in custom ML at level 70, no associativity) : ML_scope.
+Notation "x < y" := (T_BOp Lt x y)
+                      (in custom ML at level 70, no associativity) : ML_scope.
+Notation "x = y" := (T_BOp Eq x y)
+                      (in custom ML at level 70, no associativity) : ML_scope.
+
+Notation "x <> y" := (T_UOp Neg (T_BOp Eq x y))
+                       (in custom ML at level 70, no associativity) : ML_scope.
+
+Notation "x && y" := (T_BOp And x y) (in custom ML at level 80, left associativity) : ML_scope.
+Notation "x || y" := (T_BOp Or x y) (in custom ML at level 80, left associativity) : ML_scope.
+
+Notation "'~' b" := (T_UOp Neg b) (in custom ML at level 75, right associativity) : ML_scope.
+
+Notation "x + y" := (T_BOp Plus x y) (in custom ML at level 50, left associativity) : ML_scope.
+Notation "x - y" := (T_BOp Minus x y) (in custom ML at level 50, left associativity) : ML_scope.
+Notation "x * y" := (T_BOp Mult x y) (in custom ML at level 40, left associativity) : ML_scope.
+
+Notation "'inl' T t" := (T_Inl T t) (in custom ML at level 0,
+                              T custom ML_ty at level 0,
+                              t custom ML at level 0).
+Notation "'inr' T t" := (T_Inr T t) (in custom ML at level 0,
+                              T custom ML_ty at level 0,
+                              t custom ML at level 0).
+Notation "'case' t 'of' '|' 'inl' x1 '=>' t1 '|' 'inr' x2 '=>' t2" :=
+  (T_Case t x1 t1 x2 t2) (in custom ML at level 89,
+        t custom ML at level 99,
+        x1 custom ML at level 99,
+        t1 custom ML at level 99,
+        x2 custom ML at level 99,
+        t2 custom ML at level 99,
+        left associativity).
+
+
+Notation "( x ',' y )" := (T_Pair x y) (in custom ML at level 0,
+                                x custom ML at level 99,
+                                y custom ML at level 99).
+Notation "t '.1'" := (T_Fst t) (in custom ML at level 1).
+Notation "t '.2'" := (T_Snd t) (in custom ML at level 1).
+
+(* antiquotation *)
+
+Notation "{ x }" := x (in custom ML at level 1, x constr).
+
+Coercion T_Var : string >-> term.
+Coercion T_Nat : nat >-> term.
+Coercion T_Bool : bool >-> term.
+
+Open Scope ML_scope.
+
+(** We define some commonly used variables. *)
+
+Definition x : string := "x".
+Definition y : string := "y".
+Definition z : string := "z".
+
+(** ** Operational Semantics *)
+
+(** *** Values *)
+
+Inductive value : term -> Prop :=
+(* Functions *)
+| V_Fun :
+  forall x T t,
+    value <[ fun x : T -> t ]>
+(* Natural Numbers *)
+| V_Nat :
+  forall (n : nat),
+    value <[ n ]>
+(* Booleans *)
+| V_Bool :
+  forall (b : bool),
+    value <[ b ]>
+(* Sums *)
+| V_Inl : forall v T1,
+    value v ->
+    value <[ inl T1 v ]>
+| V_Inr : forall v T1,
+    value v ->
+    value <[ inr T1 v ]>
+(* Pairs *)
+| V_Pair : forall v1 v2,
+    value v1 ->
+    value v2 ->
+    value <[ (v1, v2) ]>.
+
+
+(** *** Substitution. *)
+
+Reserved Notation "'[' x ':=' s ']' t" (in custom ML at level 20, x constr).
+
+Fixpoint subst (x : string) (t' : term) (t : term) : term :=
+  match t with
+  (* pure stlc *)
+  | T_Var y =>
+      if String.eqb x y then t' else t
+  | <[ fun y : T -> t1 ]> =>
+      if String.eqb x y then t else <[ fun y : T -> [x:=t']t1 ]>
+  | <[ t1 t2 ]> =>
+      <[ ([x:=t'] t1) ([x:=t'] t2) ]>
+  (* nats and bools *)
+  | T_Nat _ => t
+  | T_Bool _ => t
+  | T_BOp bop t1 t2 => T_BOp bop <[ [x:=t'] t1 ]>  <[ [x:=t'] t2 ]>
+  | T_UOp uop t1 => T_UOp uop <[ [x:=t'] t1 ]> 
+  | <[ if t1 then t2 else t3 ]> =>
+      <[ if [x := t'] t1 then [x := t'] t2 else [x := t'] t3 ]>
+  (* pairs *)
+  | <[ (t1, t2) ]> => <[ ([x:=t'] t1, [x:=t'] t2) ]>
+  | <[ t.1 ]> => <[ ([x:=t'] t).1 ]>
+  | <[ t.2 ]> => <[ ([x:=t'] t).2 ]>
+  (* sums *)
+  | <[ inl T2 t1 ]> =>
+      <[ inl T2 ([x:=t'] t1) ]>
+  | <[ inr T1 t2 ]> =>
+      <[ inr T1 ( [x:=t'] t2) ]>
+  | <[ case t of | inl y1 => t1 | inr y2 => t2 ]> =>
+      let t1' := if String.eqb x y1 then t1 else <[ [x:=t'] t1 ]> in
+      let t2' := if String.eqb x y2 then t2 else <[ [x:=t'] t2 ]> in
+      <[ case ([x:=t'] t) of
+         | inl y1 => t1'
+         | inr y2 => t2' ]>        
+  | <[ let y := t1 in t2 ]> =>
+      let t2' := if String.eqb x y then t2 else <[ [x:=t'] t2 ]> in
+      <[ let y := [x:=t'] t1 in t2' ]>
+  end
+where "'[' x ':=' s ']' t" := (subst x s t) (in custom ML).
+
+Reserved Notation "t '-->' t'" (at level 40).
+
+(** Helper functions to distinguish between operators of different
+    types and define their interpretation. *)
+
+Definition is_nat_op (op : bop) : bool :=
+  match op with
+  | Plus | Minus | Mult => true
+  | _ => false
+  end.
+
+Definition nat_op (op : bop) : option (nat -> nat -> nat) :=
+  match op with
+  | Plus => Some add
+  | Minus => Some sub
+  | Mult => Some mul
+  | _ => None
+  end.
+
+Definition is_bool_op (op : bop) : bool :=
+  match op with
+  | And | Or => true
+  | _ => false
+  end.
+
+Definition bool_op (op : bop) : option (bool -> bool -> bool) :=
+  match op with
+  | And => Some andb
+  | Or => Some orb
+  | _ => None
+  end.
+
+Definition is_cmp_op (op : bop) : bool :=
+  match op with
+  | Eq | Lt => true
+  | _ => false
+  end.
+
+Definition cmp_op (op : bop) : option (nat -> nat -> bool) :=
+  match op with
+  | Eq => Some eqb
+  | Lt => Some ltb
+  | _  => None
+  end.
+
+(** Call-by-value reduction relation *)
+Inductive step : term -> term -> Prop :=
+(* pure STLC *)
+| Step_AppAbs : forall x T2 t1 v2,
+    value v2 ->
+    <[ (fun x:T2 -> t1) v2 ]> --> <[ [x:=v2]t1 ]>
+| Step_App1 : forall t1 t1' t2,
+    t1 --> t1' ->
+    <[ t1 t2 ]> --> <[ t1' t2 ]>
+| Step_App2 : forall v1 t2 t2',
+    value v1 ->
+    t2 --> t2' ->
+    <[ v1 t2 ]> --> <[ v1 t2' ]>
+(* Let *)
+| Step_LetVal : forall y v1 t2,
+    value v1 ->
+    <[ let y := v1 in t2 ]> --> <[ [y := v1] t2 ]>
+| Step_Let : forall y t1 t1' t2,
+    t1 --> t1'  ->
+    <[ let y := t1 in t2 ]> --> <[ let y := t1' in t2 ]>
+(* If then else *)
+| Step_IfTrue : forall t1 t2,
+    <[ if true then t1 else t2 ]> --> t1
+| Step_IfFalse : forall t1 t2,
+    <[ if false then t1 else t2 ]> --> t2
+| Step_If: forall t t' t1 t2,
+    t --> t' ->
+    <[ if t then t1 else t2 ]> --> <[ if t' then t1 else t2 ]>
+(* Binary Operators *)
+| Step_BOpNat :
+  forall bop (n1 n2 : nat) bop_f,
+    nat_op bop = Some bop_f -> 
+    (T_BOp bop n1 n2) --> T_Nat (bop_f n1 n2)
+| Step_BOpBool :
+  forall bop (b1 b2 : bool) bop_f,
+    bool_op bop = Some bop_f -> 
+    (T_BOp bop b1 b2) --> T_Bool (bop_f b1 b2)
+| Step_BOpCmp :
+  forall bop (n1 n2 : nat) bop_f,
+    cmp_op bop = Some bop_f -> 
+    (T_BOp bop n1 n2) --> T_Bool (bop_f n1 n2)
+| Step_Bop1 : forall bop t1 t1' t2,
+    t1 --> t1' ->
+    (T_BOp bop t1 t2) --> (T_BOp bop t1' t2)  
+| Step_Bop2 : forall bop v1 t2 t2',
+    value v1 ->    
+    t2 --> t2' ->
+    (T_BOp bop v1 t2) --> (T_BOp bop v1 t2')
+(* Unary Operators *)
+| Step_UOpBool : forall (b : bool),
+    (T_UOp Neg b) --> T_Bool (negb b)
+| Step_UOp : forall t t',
+    t --> t' ->
+    (T_UOp Neg t) --> (T_UOp Neg t')
+(* Pairs *)
+| Step_Pair1 : forall t1 t1' t2,
+    t1 --> t1' ->
+    <[ (t1, t2) ]> --> <[ (t1', t2) ]>
+| Step_Pair2 : forall v1 t2 t2',
+    value v1 ->
+    t2 --> t2' ->
+    <[ (v1, t2) ]> --> <[ (v1, t2') ]>
+| Step_FstPair : forall v1 v2, 
+    value v1 -> value v2 ->
+    <[ (v1, v2).1 ]> --> <[ v1 ]>
+| Step_Fst : forall t t', 
+    t --> t' ->
+    <[ t.1 ]> --> <[ t'.1 ]>
+| Step_SndPair : forall v1 v2, 
+    value v1 -> value v2 ->
+    <[ (v1, v2).2 ]> --> <[ v2 ]>
+| Step_Snd : forall t t', 
+    t --> t' ->
+    <[ t.2 ]> --> <[ t'.2 ]>
+(* sums *)
+| Step_Inl : forall t1 t1' T2,
+    t1 --> t1' ->
+    <[ inl T2 t1 ]> --> <[ inl T2 t1' ]>
+| Step_Inr : forall t2 t2' T1,
+    t2 --> t2' ->
+    <[ inr T1 t2 ]> --> <[ inr T1 t2' ]>
+| Step_Case : forall t t' x1 t1 x2 t2,
+    t --> t' ->
+    <[ case t of | inl x1 => t1 | inr x2 => t2 ]> -->
+    <[ case t' of | inl x1 => t1 | inr x2 => t2 ]>
+| Step_CaseInl : forall v x1 t1 x2 t2 T2,
+    value v ->
+    <[ case inl T2 v of | inl x1 => t1 | inr x2 => t2 ]> --> <[ [x1:=v]t1 ]>
+| Step_CaseInr : forall v x1 t1 x2 t2 T1,
+    value v ->
+    <[ case inr T1 v of | inl x1 => t1 | inr x2 => t2 ]> --> <[ [x2:=v]t2 ]>
+where "t '-->' t'" := (step t t').
+
+(** ** Typing *)
+
+(** To formalize typing we define a partial map data type to use
+    for typing environments. We represent environments as functions
+    from strings (identifiers) to optional values. We define
+    operations and notations. *)
+
+Definition partial_map A := string -> option A.
+
+Definition empty {A : Type} : partial_map A :=
+  fun _ => None.
+
+Definition update {A : Type} (m : partial_map A)
+           (x : string) (v : A) :=
+  fun x' => if String.eqb x x' then Some v else m x'.
+
+Notation "x '|->' v ';' m" := (update m x v)
+  (at level 100, v at next level, right associativity).
+
+Notation "x '|->' v" := (update empty x v)
+  (at level 100).
+
+(** The type of typing environments. *)
+Definition context := string -> option type.
+
+Reserved Notation "Gamma '⊢' t ':' T" (at level 40, t custom ML, T custom ML_ty at level 0).
+
+(* The typing relation *)
+Inductive has_type : context -> term -> type -> Prop :=
+  (* Pure STLC *)
+  | Ty_Var : forall Gamma x A,
+      Gamma x = Some A ->
+      Gamma ⊢ x : A
+  | Ty_Abs : forall Gamma x t A B ,
+      (x |-> A ; Gamma) ⊢ t : B ->
+      Gamma ⊢ (fun x : A -> t) : (A -> B)
+  | Ty_App : forall Gamma t1 t2 A B,
+      Gamma ⊢ t1 : (A -> B) ->
+      Gamma ⊢ t2 : A ->
+      Gamma ⊢ t1 t2 : B
+  (* Let *)
+  | Ty_Let : forall Gamma x t1 t2 A B,
+      Gamma ⊢ t1 : A ->
+      (x |-> A ; Gamma) ⊢ t2 : B ->
+      Gamma ⊢ (let x := t1 in t2) : B
+  (* Bools *)
+  | Ty_Bool : forall Gamma (b : bool),
+      Gamma ⊢ b : Bool
+  | Ty_If : forall Gamma t1 t2 t3 A,
+      Gamma ⊢ t1 : Bool ->
+      Gamma ⊢ t2 : A ->
+      Gamma ⊢ t3 : A ->
+      Gamma ⊢ if t1 then t2 else t3 : A
+  | Ty_BopBool : forall Gamma bop t1 t2,
+      Gamma ⊢ t1 : Bool ->
+      Gamma ⊢ t2 : Bool ->
+      is_bool_op bop = true ->
+      Gamma ⊢ { T_BOp bop t1 t2 } : Bool
+  | Ty_UOp : forall Gamma uop t1,
+      Gamma ⊢ t1 : Bool ->
+      Gamma ⊢ { T_UOp uop t1 } : Bool
+  (* Numbers *)
+  | Ty_Nat : forall Gamma (n : nat),
+      Gamma ⊢ n : Nat
+  | Ty_BopNat : forall Gamma bop t1 t2,
+      Gamma ⊢ t1 : Nat ->
+      Gamma ⊢ t2 : Nat ->
+      is_nat_op bop = true ->
+      Gamma ⊢ { T_BOp bop t1 t2 } : Nat
+  | Ty_BopCmp : forall Gamma bop t1 t2,
+      Gamma ⊢ t1 : Nat ->
+      Gamma ⊢ t2 : Nat ->
+      is_cmp_op bop = true ->
+      Gamma ⊢ { T_BOp bop t1 t2 } : Bool
+  (* Pairs *)
+  | Ty_Pair : forall Gamma t1 t2 A B,
+      Gamma ⊢ t1 : A ->
+      Gamma ⊢ t2 : B ->
+      Gamma ⊢ (t1, t2) : (A * B)
+  | Ty_Fst : forall Gamma t1 A B,
+      Gamma ⊢ t1 : (A * B) ->
+      Gamma ⊢ t1.1 : A
+  | Ty_Snd : forall Gamma t1 (A B : type),
+      Gamma ⊢ t1 : (A * B) ->
+      Gamma ⊢ t1.2 : B
+  (* Sums *)
+  | Ty_Inl : forall Gamma t1 A B,
+      Gamma ⊢ t1 : A ->
+      Gamma ⊢ (inl B t1) : (A + B)
+  | Ty_Inr : forall Gamma t2 A B,
+      Gamma ⊢ t2 : B ->
+      Gamma ⊢ (inr A t2) : (A + B)
+  | Ty_Case : forall Gamma t x1 A t1 x2 B t2 C,
+      Gamma ⊢ t : (A + B) ->
+      (x1 |-> A ; Gamma) ⊢ t1 : C ->
+      (x2 |-> B ; Gamma) ⊢ t2 : C ->
+      Gamma ⊢ (case t of | inl x1 => t1 | inr x2 => t2) : C
+where "Gamma '⊢' t ':' T" := (has_type Gamma t T).
+
+
+(** We extend the auto core database with the constructors of the
+    [value], [step] and [has_type] relations. *)
+
+Hint Constructors value : core.
+Hint Constructors step : core.
+Hint Constructors has_type : core.
+
+(** ** Type Safety **)
+
+Ltac inv H := inversion H; clear H; subst.
+
+(** We can now move on to the proof of progress and preservation. *)
+
+(** *** Canonical Forms *)
+
+(** We first prove a series of _canonical forms_ lemmas.  They state
+    that if a term that is a value has a certain type, then it must be
+    a value of that type. They are proved by straightforward inversion
+    of the value and typing relations. *)
+
+Lemma canonical_forms_bool :
+  forall t,
+    empty ⊢ t : Bool ->
+    value t ->
+    (t = <[ true ]>) \/ (t = <[ false ]>).
+Proof.
+  intros t Htyp Hval.
+  inv Hval; inv Htyp.
+  destruct b; auto.
+Qed.
+
+Lemma canonical_forms_nat :
+  forall t,
+    empty ⊢ t : Nat ->
+    value t ->
+    exists (n : nat), t = <[ n ]>.
+Proof.
+  intros t Htyp Hval.
+  inv Hval; inv Htyp. eauto.
+Qed.
+
+Lemma canonical_forms_fun :
+  forall t T1 T2,
+    empty ⊢ t : (T1 -> T2) ->
+    value t ->
+    exists x u, t = <[ fun x : T1  -> u ]>.
+Proof.
+  intros t T1 T2 Htyp Hval.
+  inv Hval; inv Htyp. eauto.
+Qed.
+
+Lemma canonical_forms_sum :
+  forall t T1 T2,
+    empty ⊢ t : (T1 + T2) ->
+    value t ->
+    (exists t1, t = <[ inl T2 t1 ]> /\ value t1) \/
+    (exists t2, t = <[ inr T1 t2 ]> /\ value t2).
+Proof.
+  intros t T1 T2 Htyp Hval.
+  inv Hval; inv Htyp; eauto.
+Qed.
+
+Lemma canonical_forms_prod :
+  forall t T1 T2,
+    empty ⊢ t : (T1 * T2) ->
+    value t ->
+    exists t1 t2, t = <[ (t1, t2) ]> /\ value t1 /\ value t2.
+Proof.
+  intros t T1 T2 Htyp Hval.
+  inv Hval; inv Htyp; eauto.
+Qed.
+
+(** Helper lemmas for binary operators *)
+
+Lemma is_nat_op_lemma :
+  forall bop, is_nat_op bop = true -> exists f, nat_op bop = Some f. 
+Proof. intros []; simpl; try discriminate; eauto. Qed.
+
+Lemma is_bool_op_lemma :
+  forall bop, is_bool_op bop = true -> exists f, bool_op bop = Some f. 
+Proof. intros []; simpl; try discriminate; eauto. Qed.
+
+Lemma is_cmp_op_lemma :
+  forall bop, is_cmp_op bop = true -> exists f, cmp_op bop = Some f. 
+Proof. intros []; simpl; try discriminate; eauto. Qed.
+
+(** *** Progress *)
+
+(** Note: Proof of certain cases and comments are taken from "Software
+    Foundations"*)
+
+(** Theorem: Suppose empty ⊢- t \in A.  Then either
+      1. t is a value, or
+      2. t --> t' for some t'.
+
+    Proof: By induction on the given typing derivation. *)
+
+Theorem progress : forall t T,
+     empty ⊢ t : T ->
+     value t \/ exists t', t --> t'.
+Proof.
+  intros t T Ht.
+  remember empty as Gamma.
+  induction Ht; subst.
+  - (* Ty_Var *)
+    (* The final rule in the given typing derivation cannot be
+       [T_Var], since it can never be the case that
+       [empty ⊢ x : T] (since the context is empty). *)
+    discriminate H.    
+  - (* Ty_Abs *)
+    (* If the [Ty_Abs] rule was the last used, then
+       [t = fun x0 : T2 -> t1], which is a value. *)
+    now left.
+    
+  - (* Ty_App *)
+    
+    (* If the last rule applied was Ty_App, then [t = t1 t2],
+       and we know from the form of the rule that
+         [empty ⊢ t1 : T1 -> T2]
+         [empty ⊢ t2 : T1]
+       By the induction hypothesis, each of t1 and t2 either is
+       a value or can take a step. *)
+    right.
+    
+    destruct IHHt1.
+    + reflexivity.
+    + (* t1 is a value *)
+      destruct IHHt2.
+      * reflexivity.
+      * (* t2 is a value *)
+        (* If both [t1] and [t2] are values, then we know that
+           [t1 = fun x0 : T0 -> t11], since abstractions are the
+           only values that can have an arrow type.  But
+           [(fun x0 : T0 -> t11) t2 --> [x:=t2]t11] by [ST_AppAbs]. *)
+        eapply canonical_forms_fun in Ht1; [| assumption ].
+
+        destruct Ht1 as [x [u Heq]]; subst.
+        eauto.        
+      * (* t2 steps *)
+        (* If [t1] is a value and [t2 --> t2'],
+           then [t1 t2 --> t1 t2'] by [ST_App2]. *)
+        destruct H0 as [t2' Hstp].        
+        exists <[t1 t2']>; auto.
+    + (* t1 steps *)
+      (* Finally, If [t1 --> t1'], then [t1 t2 --> t1' t2]
+         by [ST_App1]. *)
+      destruct H as [t1' Hstp]. exists <[t1' t2]>; auto.
+  - (* Ty_let *)
+    destruct IHHt1 as [ | [t1' Hstp]];
+      subst; [ reflexivity | now eauto | now eauto ]. 
+  - (* Ty_Bool *)
+    eauto.
+
+  - (* TY_If *)
+    destruct IHHt1 as [ | [t1' Hstp]];
+      subst; [ reflexivity | | now eauto ].
+
+    edestruct (canonical_forms_bool t1); subst; eauto.
+
+  - (* Ty_Bop bool *)
+    destruct IHHt1 as [ | [t1' Hstp]];
+      subst; [ reflexivity | | now eauto ]. 
+    destruct IHHt2 as [ | [t2' Hstp]];
+      subst; [ reflexivity | | now eauto ]. 
+
+    edestruct is_bool_op_lemma; eauto.
+
+    edestruct (canonical_forms_bool t1); eauto; subst;
+    edestruct (canonical_forms_bool t2); eauto; subst; eauto.
+
+  - (* T_Uop bool *)
+    destruct uop0.
+    destruct IHHt as [ | [t1' Hstp]];
+      subst; [ reflexivity | | now eauto]. 
+     
+    edestruct (canonical_forms_bool t1); eauto; subst; eauto.
+
+  - (* Ty_Nat *)
+    left; auto.
+  - destruct IHHt1 as [ | [t1' Hstp]];
+      subst; [ reflexivity | | now eauto ]. 
+    destruct IHHt2 as [ | [t2' Hstp]];
+      subst; [ reflexivity | | now eauto ]. 
+
+    edestruct (canonical_forms_nat t1); eauto; subst.
+    edestruct (canonical_forms_nat t2); eauto; subst.
+
+    edestruct is_nat_op_lemma; eauto.
+
+  - (* Ty_Bop cmp *)
+    destruct IHHt1 as [ | [t1' Hstp]];
+      subst; [ reflexivity | | now eauto ]. 
+    destruct IHHt2 as [ | [t2' Hstp]];
+      subst; [ reflexivity | | now eauto ]. 
+
+    edestruct (canonical_forms_nat t1); eauto; subst.
+    edestruct (canonical_forms_nat t2); eauto; subst.
+
+    edestruct is_cmp_op_lemma; eauto.
+
+  - (* Ty_Pair *)
+    destruct IHHt1 as [ | [t1' Hstp]];
+      subst; [ reflexivity | | now eauto ]. 
+    destruct IHHt2 as [ | [t2' Hstp]];
+      subst; [ reflexivity | | now eauto ]. 
+
+    eauto.
+    
+  - (* Ty_fst *)
+    destruct IHHt as [ | [t' Hstp]];
+      subst; [ reflexivity | | now eauto ].
+    edestruct (canonical_forms_prod t1) as [ v1 [v2 [Hstp1 [Hv1 Hv2]]]]; eauto.
+    subst; eauto.
+
+  - (* Ty_snd *)
+    destruct IHHt as [ | [t' Hstp]];
+      subst; [ reflexivity | | now eauto ].
+    edestruct (canonical_forms_prod t1) as [ v1 [v2 [Hstp1 [Hv1 Hv2]]]]; eauto.
+    subst; eauto.
+
+      - (* Ty_Inl *)
+    destruct IHHt as [ | [t1' Hstp]];
+      subst; [ reflexivity | now eauto | now eauto ]. 
+
+  - (* Ty_Inr *)
+    destruct IHHt as [ | [t1' Hstp]];
+      subst; [ reflexivity | now eauto | now eauto ].
+
+  - (* Ty_case *)
+    destruct IHHt1 as [ | [t1' Hstp]];
+      subst; [ reflexivity | | now eauto ].
+
+    edestruct (canonical_forms_sum t) as [ [v1 [Hstp1 Hv1]] | [v2 [Hstp2 Hv2]]];
+      eauto; subst; eauto.
+
+Qed.
+
+
+(** *** Weakening *)
+
+(** In order to prove preservation, we first need to prove a weakening
+    lemma. That is, if [Gamma ⊢ t : A], then [Gamma' ⊢ t : A], for any
+    [Gamma'] that contains all the bindings of [Gamma], and possibly
+    more. *)
+
+(** We formalize a notion of submap. A map [m] is a submap of [m'], if
+    any mapping [x |-> v] that is in [m] is also in [m'].  *)
+
+Definition submap {A : Type} (m m' : partial_map A) : Prop :=
+  forall x v, m x = Some v -> m' x = Some v.
+
+(** We prove some useful lemmas for maps and the submap relation. *)
+
+Lemma update_eq : forall (A : Type) (m : partial_map A) x v,
+  (x |-> v ; m) x = Some v.
+Proof.
+  intros. unfold update. rewrite eqb_refl. reflexivity.
+Qed.
+
+Theorem update_neq : forall (A : Type) (m : partial_map A) x1 x2 v,
+  x2 <> x1 ->
+  (x2 |-> v ; m) x1 = m x1.
+Proof.
+  intros A m x1 x2 v H.
+  unfold update.
+  apply eqb_neq in H. rewrite H. reflexivity.
+Qed.
+
+Lemma submap_update :
+  forall (A : Type) (m m' : partial_map A) (x : string) (vx : A),
+  submap m m' ->
+  submap (x |-> vx ; m) (x |-> vx ; m').
+Proof.
+  unfold submap.
+  intros A m m' x vx H.
+  intros y vy.
+  destruct (eqb_spec x y) as [Hxy | Hxy].
+  - rewrite Hxy.
+    rewrite update_eq. rewrite update_eq. intro H1. apply H1.
+  - rewrite update_neq.
+    + rewrite update_neq.
+      * apply H.
+      * apply Hxy.
+    + apply Hxy.
+Qed.
+
+
+(** Weakening follows easily by induction on the typing derivation. *)
+
+Lemma weakening :
+  forall Gamma Gamma' t A,
+    submap Gamma Gamma' ->
+    Gamma  ⊢ t : A  ->
+    Gamma' ⊢ t : A.
+Proof.
+  intros Gamma Gamma' t  A Hsub Ht.
+  revert Gamma' Hsub.
+  induction Ht; eauto 7 using submap_update.
+Qed.
+
+Corollary weakening_empty :
+  forall Gamma t A,
+    empty ⊢ t : A  ->
+    Gamma ⊢ t : A.
+Proof.
+  intros Gamma t A.
+  eapply weakening.
+  discriminate.
+Qed.
+
+
+(** *** Substitution Preserves Typing *)
+
+(** Another crucial lemma that we will use is that substitution
+    preserves typing. This lemma says that if
+
+    [(x |-> B ; Gamma) ⊢ t : A]
+
+    then we can substitute any closed term of type [B] for [x], and
+    the resulting term will still have type [A]. That is, 
+ 
+    if [empty ⊢ v : B] then [Gamma ⊢ [x:=v]t : A].
+*)
+
+
+(** Before proceeding, we need to establish some intuitive properties
+    about partial maps. To do so, we will rely on the axiom of
+    functional extensionality. This axiom states that two functions
+    are equal if they produce the same output for all inputs:
+
+    [forall f g, (forall x, f x = g x) -> f = g]
+
+    This intuitive statement cannot be directly proven using the
+    standard definition of equality in Coq, which requires syntactic
+    equality. However, adding this axiom is logically sound and
+    simplifies reasoning about functions.
+
+   It is worth noting that we could have proved preservation without
+   invoking functional extensionality, but the resulting proof would
+   be more cumbersome and tedious. By using this axiom, we streamline
+   the process while maintaining the rigor of our reasoning. *)
+
+Require Import Coq.Logic.FunctionalExtensionality. 
+
+Check functional_extensionality.
+
+Lemma update_shadow :
+  forall (A : Type) (m : partial_map A) x v1 v2,
+    (x |-> v2 ; x |-> v1 ; m) = (x |-> v2 ; m).
+Proof.
+  intros A m x v1 v2. unfold update.
+  apply functional_extensionality. intros y.
+  destruct (eqb_spec x y); subst; eauto.
+Qed.
+
+Lemma update_same :
+  forall (A : Type) (m : partial_map A) x v,
+    m x = Some v ->
+    (x |-> v ; m) = m.
+Proof.
+  intros A m x v H. unfold update. rewrite <- H.
+  apply functional_extensionality. intros y.
+  destruct (eqb_spec x y); subst; eauto.
+Qed.
+
+Lemma update_permute :
+  forall (A : Type) (m : partial_map A) x1 x2 v1 v2,
+    x2 <> x1 ->
+    (x1 |-> v1 ; x2 |-> v2 ; m) = (x2 |-> v2 ; x1 |-> v1 ; m).
+Proof.
+  intros A m x1 x2 v1 v2 Hneq. unfold update.
+  apply functional_extensionality. intros y.
+  destruct (eqb_spec x1 y); subst; eauto.
+  destruct (eqb_spec x2 y); subst; eauto.
+  congruence. 
+Qed.
+
+(** Substitution preserves typing lemma. *)
+
+Lemma substitution_preserves_typing :
+  forall Gamma x v t A B,
+    (x |-> B ; Gamma) ⊢ t : A ->
+    empty ⊢ v : B   ->
+    Gamma ⊢ [x:=v]t : A.
+Proof.
+  intros Gamma x v t A B Ht Hv.
+  revert Gamma A Ht Hv. 
+  induction t; intros Gamma A Ht1 Ht2; inv Ht1; simpl; eauto.
+  - (* T_Abs *)
+    destruct (eqb_spec x s); subst; apply Ty_Abs.
+    + (* x = s *)
+      rewrite update_shadow in H4. assumption.
+    + (* x <> s *)
+      apply IHt; auto.
+      rewrite update_permute; auto.
+
+  - (* T_Var *)
+    destruct (eqb_spec x s); subst.
+    + (* x = s *)
+      rewrite update_eq in H1. inv H1. 
+      apply weakening_empty. assumption.
+    + (* x <> y *)
+      apply Ty_Var. rewrite update_neq in H1; auto.
+
+  - (* T_let *)
+    eapply Ty_Let.
+    + eapply IHt1; eauto.
+    + destruct (eqb_spec x s); subst.
+      * (* x = s *)        
+        rewrite update_shadow in H5. assumption.
+      * (* x <> s *)        
+        eapply IHt2; auto.
+        rewrite update_permute; eauto.
+  - (* T_Case *)
+    eapply Ty_Case.
+    + now eauto.
+    + destruct (eqb_spec x s); subst.
+      * (* x = s *)
+        rewrite update_shadow in H7. assumption.
+      * (* x <> s *)
+        apply IHt2.
+        rewrite update_permute; auto.
+        assumption.
+    + destruct (eqb_spec x s0); subst.
+      * (* x = s0 *)
+        rewrite update_shadow in H8. assumption.
+      * (* x <> s0 *)
+        apply IHt3.
+        rewrite update_permute; auto.
+        assumption.
+Qed.
+
+(** *** Preservation *)
+
+(** We can now prove the preservation theorem. *)
+
+Theorem preservation :
+  forall t t' A,
+    empty ⊢ t : A  ->
+    t --> t'  ->
+    empty ⊢ t' : A.
+Proof.
+  intros t t' A Htyp. revert t'.
+  remember empty as Gamma.
+  induction Htyp; intros t' Hstep; subst.
+  - (* Ty_Var *)
+    inv Hstep.
+  - (* Ty_Abs *)
+    inv Hstep.
+  - (* Ty_App *)
+    inv Hstep.
+    inv Htyp1.
+    + eapply substitution_preserves_typing; eauto.
+    + eauto.
+    + eauto.
+
+  - (* Ty_Let *)
+    inv Hstep; eauto.
+    eapply substitution_preserves_typing; eauto.
+
+  - (* Ty_Bool *)
+    inv Hstep.
+
+  - (* Ty_If *)
+    inv Hstep; eauto.
+
+  - (* Ty_Bop *)
+    inv Hstep; eauto.
+    
+    now destruct bop0; simpl in *; try congruence. (* TODO nicer *)
+
+  - (* Ty_UOp *)
+    inv Hstep; eauto.
+
+  - (* Ty_Nat *)
+    inv Hstep.
+
+  - (* Ty_Bop *)
+    inv Hstep; eauto.
+
+    now destruct bop0; simpl in *; try congruence.
+
+    now destruct bop0; simpl in *; try congruence. (* TODO nicer *)
+
+  - (* Ty_Bop *)
+    inv Hstep; eauto.
+
+    now destruct bop0; simpl in *; try congruence. (* TODO nicer *)
+
+  - (* Ty_Pair *)
+    inv Hstep; eauto.
+
+  - (* Ty_Fst *)
+    inv Hstep; eauto.
+    
+    inv Htyp; eauto. 
+
+  - (* Ty_Snd *)
+    inv Hstep; eauto.
+    
+    inv Htyp; eauto. 
+
+  - (* Ty_inl *)
+    inv Hstep; eauto.
+    
+  - (* Ty_inr *)
+    inv Hstep; eauto.
+    
+  - (* Ty_case *)
+    inv Hstep; eauto.
+    + inv Htyp1.
+      eapply substitution_preserves_typing; eauto.
+    + inv Htyp1. 
+      eapply substitution_preserves_typing; eauto.
+
+Qed. 
+
+
+(** ** Type Checking *)
+
+(** Lastly, we define a typechecking program that we prove sound and
+    complete with respect to our typing relation. *)
+
+
+(** First, we define equality on types by recursion on their
+    structure. *)
+Fixpoint ty_eqb (A B: type) : bool :=
+  match A, B with
+  | Bool, Bool => true
+  | Nat, Nat => true
+  | Unit, Unit => true
+  | <[[ A1 -> A2 ]]>, <[[ B1 -> B2 ]]> =>
+      andb (ty_eqb A1 B1) (ty_eqb A2 B2)
+  | <[[ A1 + A2 ]]>, <[[ B1 + B2 ]]> =>
+      andb (ty_eqb A1 B1) (ty_eqb A2 B2)
+  | <[[ A1 * A2 ]]>, <[[ B1 * B2 ]]> =>
+      andb (ty_eqb A1 B1) (ty_eqb A2 B2)
+  | _, _ => false
+  end.
+
+
+(** The typechecking function is defined by induction on the input term
+    and returns either some type (the type of the term) or nothing ([None]),
+    if the term is not well-typed. *)
+
+(** To avoid boilerplate code when writing a function that manipulates
+    a lot of [option] types, we introduce a so called _monadic_
+    notation for sequencing operations.
+
+    The sequencing operation [x <- e1 ;; e2] evaluates [e1] and if it
+    returns some value, then it binds it to x, and evaluates
+    [e2]. Otherwise, it propagates [None].
+
+    The _action_ [return v] "returns" [Some v], and the _action_
+    [fail] returns [None]. *)
+
+Notation "x <- e1 ;; e2" := (match e1 with
+                             | Some x => e2
+                             | None => None
+                              end)
+         (right associativity, at level 60).
+
+Notation " 'return' e " := (Some e) (at level 60).
+
+Notation " 'fail' " := None.
+
+(* Note: We will explore monads in more depth later in the course *)
+
+Fixpoint type_check (Gamma : context) (t : term) : option type :=
+  match t with
+  (*  Pure STLC *)
+  | T_Var x => Gamma x
+  | <[ fun x : A -> t1 ]> =>
+      B <- type_check (x |-> A ; Gamma) t1 ;;
+      return <[[ A -> B ]]>
+  | <[ t1 t2 ]> =>
+      A <- type_check Gamma t1 ;;
+      B <- type_check Gamma t2 ;;
+      match A with
+      | <[[ A1 -> A2 ]]> =>
+          if ty_eqb A1 B then return A2 else fail
+      | _ => fail
+      end
+  (* Let *)
+  | <[ let y := t1 in t2 ]> =>
+      A <- type_check Gamma t1 ;;
+      type_check (y |-> A ; Gamma) t2
+  (* Booleans *)
+  | T_Bool _ => return <[[ Bool ]]>
+  | <[ if b then t1 else t2 ]> =>
+      A <- type_check Gamma b ;;
+      B <- type_check Gamma t1 ;;
+      C <- type_check Gamma t2 ;;
+      match A with
+      | <[[ Bool ]]> => if ty_eqb B C then return B else fail
+      | _ => fail
+      end
+  (* Numbers *)
+  | T_Nat n => return <[[ Nat ]]>    
+  (* Binary operators *)
+  | T_BOp bop t1 t2 =>
+      A <- type_check Gamma t1 ;;
+      B <- type_check Gamma t2 ;;
+      if ty_eqb A B then 
+        if is_nat_op bop then
+          if ty_eqb A Nat then return Nat else fail
+        else if is_cmp_op bop then
+          if ty_eqb A Nat then return Bool else fail
+        else if is_bool_op bop then
+          if ty_eqb A Bool then return Bool else fail
+        else fail
+      else fail
+  (* Unary operators *)
+  | T_UOp b t1 =>
+      A <- type_check Gamma t1 ;;
+      if ty_eqb A Bool then return Bool else fail
+  (* Pairs *)
+  | <[ (t1, t2)]> =>
+      A <- type_check Gamma t1 ;;
+      B <- type_check Gamma t2 ;;
+      return <[[ A * B ]]>
+  | <[ t1.1 ]> =>
+      A <- type_check Gamma t1 ;;
+      match A with
+      | <[[ A1 * A2 ]]> => return A1
+      | _ => fail
+      end
+  | <[ t1.2 ]> =>
+      A <- type_check Gamma t1 ;;
+      match A with
+      | <[[ A1 * A2 ]]> => return A2
+      | _ => fail
+      end
+  (* Sums *)
+  | <[ inl B t1 ]> =>
+      A <- type_check Gamma t1 ;;
+      return <[[ A + B ]]>
+  | <[ inr A t1 ]> =>
+      B <- type_check Gamma t1 ;;
+      return <[[ A + B ]]>
+  | <[ case t of | inl y1 => t1 | inr y2 => t2 ]> =>
+      A <- type_check Gamma t ;;
+      match A with
+      | <[[ A1 + A2 ]]> =>
+          B <- type_check (y1 |-> A1 ; Gamma) t1 ;; 
+          C <- type_check (y2 |-> A2 ; Gamma) t2 ;;
+          if ty_eqb B C then return B else fail
+      | _ => fail
+      end
+  end.
+
+(** *** Correctness of Type Checking *)
+
+(** We first prove some simple lemmas about type equality. *)
+
+Lemma ty_eqb_eq :
+  forall t1 t2, ty_eqb t1 t2 = true -> t1 = t2.
+Proof.
+  induction t1; intros []; simpl; intros H; try congruence.
+  - apply andb_prop in H. destruct H.
+    erewrite IHt1_1; eauto.
+    erewrite IHt1_2; eauto.
+  - apply andb_prop in H. destruct H.
+    erewrite IHt1_1; eauto.
+    erewrite IHt1_2; eauto.
+  - apply andb_prop in H. destruct H.
+    erewrite IHt1_1; eauto.
+    erewrite IHt1_2; eauto.
+Qed.    
+
+Lemma ty_eqb_refl :
+  forall t, ty_eqb t t = true.
+Proof.
+  induction t; simpl; auto.
+  - rewrite IHt1; eauto.
+  - rewrite IHt1; eauto.
+  - rewrite IHt1; eauto.
+Qed.    
+
+
+Ltac simpl_tc :=
+  match reverse goal with
+  | [H: ty_eqb ?t1 ?t2 = true |- _] => apply ty_eqb_eq in H; subst
+  | [H: Some _ = Some _ |- _] => inv H
+  | [_ : match ?t with _ => _ end = _ |- _] =>
+      destruct t eqn:?; try congruence
+  | [_: context[ty_eqb ?t1 ?t2] |- _] =>
+      destruct (ty_eqb t1 t2) eqn:?; subst; try congruence
+  end.
+
+(** Soundness. *)
+Theorem type_checking_sound :
+  forall Gamma t A,
+    type_check Gamma t = Some A ->
+    Gamma ⊢ t : A.
+Proof.
+  intros Gamma t. revert Gamma.
+  induction t; intros Gamma A Htc; simpl in *;
+    try now (repeat simpl_tc; eauto).
+Qed.
+
+(** Completeness. *)
+Theorem type_checking_complete :
+  forall Gamma t A,
+    Gamma ⊢ t : A ->
+    type_check Gamma t = Some A.
+Proof.
+  intros Gamma t A Htyp; induction Htyp; simpl; eauto;
+  try rewrite IHHtyp; try rewrite IHHtyp1; try rewrite IHHtyp2;
+    try rewrite IHHtyp3;
+    try rewrite ty_eqb_refl; try reflexivity.
+  
+  - destruct bop0; simpl in *; try congruence.
+  - destruct bop0; simpl in *; try congruence.
+  - destruct bop0; simpl in *; try congruence.    
+Qed.
